\documentclass{article}
\usepackage{amsmath}
\usepackage{amssymb}
\begin{document}
Let $X: = \left( x_n \right)$ and $Y:= \left( y_n \right)$ by sequences in $\mathbb{R}$ and let the partial sums of $\sum\left( y_n \right)$ be denoted by $\left( s_)n \right)$ with $s_0 : = 0$ \\

If $m>n$, then

\begin{equation}
  \sum_{k=n+1}^{m}\left[ x_ky_k \right]=\left( x_ms_m - x_{n+1}s_n \right) + \sum{k=n+1}^{m-1}\left( x_k-x_k+1 \right)s_k
  \label{partsum}
\end{equation}


$v:=v_{\delta}\left( c \right)$

$f'\left( c \right) = \frac{f\left( b \right)-f\left( a \right)}{b-a}$
\left( b-a \right) \cdot f\left( c \right) = f\left( b \right) - f\left( a \right)


\frac{f\left( b \right)-f\left( a \right)}{g\left( b \right) - g\left( a \right)} = \frac{f'\left( c \right)}{g'\left( c \right)}

\end{document}

